simplify handling of instructions whose leakage trace has not been defined

src/riscv/Platform/MetricRiscvMachine.v
@@ -59,11 +59,11 @@ Section Machine.
     fun items '(mkMetricRiscvMachine mach mc) =>
       (mkMetricRiscvMachine (withLogItems items mach) mc).
 
-  Definition withLeakageEvent: LeakageEvent -> MetricRiscvMachine -> MetricRiscvMachine :=
+  Definition withLeakageEvent: option LeakageEvent -> MetricRiscvMachine -> MetricRiscvMachine :=
     fun event '(mkMetricRiscvMachine mach mc) =>
       (mkMetricRiscvMachine (withLeakageEvent event mach) mc).
 
-  Definition withLeakageEvents: list LeakageEvent -> MetricRiscvMachine -> MetricRiscvMachine :=
+  Definition withLeakageEvents: option (list LeakageEvent) -> MetricRiscvMachine -> MetricRiscvMachine :=
     fun events '(mkMetricRiscvMachine mach mc) =>
       (mkMetricRiscvMachine (withLeakageEvents events mach) mc).
 
