src/riscv/Platform/MinimalMMIO.v
@@ -115,10 +115,7 @@ Section Riscv.
         postF tt (withNextPc (word.add mach.(getPc) (word.of_Z 4)) mach)
     | EndCycleNormal => fun postF postA => postF tt (updatePc mach)
     | EndCycleEarly _ => fun postF postA => postA (updatePc mach) (* ignores postF containing the continuation *)
-    | LeakEvent e => fun postF postA => match e with
-                                        | Some e => postF tt (withLeakageEvent e mach)
-                                        | None => forall X (x : X), postF tt (withLeakageEvent (anything x) mach)
-                                        end
+    | LeakEvent e => fun postF postA => postF tt (withLeakageEvent e mach)
     | MakeReservation _
     | ClearReservation _
     | CheckReservation _
@@ -165,7 +162,6 @@ Section Riscv.
   Proof.
     destruct a; cbn; try solve [intuition eauto].
     all : eauto using load_weaken_post, store_weaken_post.
-    intros. destruct o; eauto.
   Qed.
 
   Global Instance MinimalMMIOSatisfies_mcomp_sat_spec: mcomp_sat_spec MinimalMMIOPrimitivesParams.
@@ -195,7 +191,6 @@ Section Riscv.
       cbv [load store nonmem_load nonmem_store]; cbn -[HList.tuple];
         repeat destruct_one_match;
         intuition idtac;
-        try match goal with | H : forall _ _, _ |- _ => specialize (H True I) end;
         repeat lazymatch goal with
                | H : postF _ ?mach |- exists _ : RiscvMachine, _ =>
                  exists mach; cbn [RiscvMachine.getMem RiscvMachine.getXAddrs]
